clib: respect exceptional control flow in `cinit` variable lifting
`cinit` and related methods are able to automatically abstract accesses
of Simpl state variables to Isabelle variables, provided they can prove
that the Simpl variable has not been modified up to the point it is
accessed. However, previously, the automation was unaware of exceptional
control flow. This limits the effectiveness of variable lifting in
situations like the following:

    // `var` has not yet been modified.
    if (condition) {
        var = new_value;
        // Here, `var` has been modified.
        return;
    }
    // Has `var` been modified before the following access?
    do_something(var);

Prior to this commit, the answer would be "yes": `cinit` would conclude
that `var` has been modified prior to the access for `do_something`, so
the variable access would not be abstracted.

With this commit, the answer is "no": `cinit` recognises the `return` in
the `if` block, and can abstract the variable access for `do_something`.

The new automation is enabled for `cinit`, `clift` and `ctac`. It is
currently disabled for `csymbr`, since the new behaviour breaks some
existing proofs.

Signed-off-by: Matthew Brecknell <Matthew.Brecknell@data61.csiro.au>

lib/clib/XPres.thy
@@ -8,258 +8,415 @@ theory XPres
 imports SIMPL_Lemmas
 begin
 
-(* We don't really care if the computation gets stuck or faults, only that xf isn't changed *)
-definition
-  xpres :: "('s \<Rightarrow> 'a) \<Rightarrow> 'a \<Rightarrow> ('i \<rightharpoonup> ('s, 'i, 'x) com) \<Rightarrow> ('s, 'i, 'x) com \<Rightarrow> bool"
-where
-  "xpres xf v \<Gamma> c \<equiv> \<forall>s t. \<Gamma> \<turnstile> \<langle>c, s\<rangle> \<Rightarrow> t
-  \<longrightarrow> s \<in> Normal ` {s. xf s = v}
-  \<longrightarrow> (\<forall>t'. t = Normal t' \<or> t = Abrupt t' \<longrightarrow> xf t' = v)"
+(* FIXME: move *)
+lemmas trivial = TrueE[OF TrueI]
+
+(* Intended to be used to calculate `z` from `b`, `x` and `y`. *)
+definition xpres_eq_If :: "bool \<Rightarrow> 'a \<Rightarrow> 'a \<Rightarrow> 'a \<Rightarrow> bool" where
+  "xpres_eq_If b x y z \<equiv> z = (if b then x else y)"
+
+lemma xpres_eq_If_False:
+  "xpres_eq_If False x y y"
+  by (simp add: xpres_eq_If_def)
+
+lemma xpres_eq_If_True:
+  "xpres_eq_If True x y x"
+  by (simp add: xpres_eq_If_def)
+
+lemmas xpres_eq_If_rules = xpres_eq_If_False xpres_eq_If_True
+
+(* Intended to be used to calculate `abnormal` by syntactic analysis of `c`. *)
+definition xpres_abnormal where
+  "xpres_abnormal \<Gamma> c abnormal \<equiv> \<forall>s t. abnormal \<longrightarrow> \<not> \<Gamma> \<turnstile> \<langle>c, Normal s\<rangle> \<Rightarrow> Normal t"
+
+lemma xpres_abnormalD:
+  assumes "xpres_abnormal \<Gamma> c abnormal"
+  assumes "abnormal"
+  assumes "\<Gamma> \<turnstile> \<langle>c, Normal s\<rangle> \<Rightarrow> Normal t"
+  shows False
+  using assms by (auto simp: xpres_abnormal_def)
+
+lemma xpres_abnormalI:
+  assumes "\<And>s t. \<lbrakk>abnormal; \<Gamma> \<turnstile> \<langle>c, Normal s\<rangle> \<Rightarrow> Normal t\<rbrakk> \<Longrightarrow> False"
+  shows "xpres_abnormal \<Gamma> c abnormal"
+  using assms by (auto simp: xpres_abnormal_def)
+
+lemma xpres_abnormal_trivial:
+  "xpres_abnormal \<Gamma> c False"
+  by (auto simp: xpres_abnormal_def)
+
+lemma xpres_abnormal_throw:
+  "xpres_abnormal \<Gamma> Throw True"
+  by (auto simp: xpres_abnormal_def elim!: exec_elim_cases)
+
+lemma xpres_abnormal_creturn:
+  "xpres_abnormal \<Gamma> (creturn rtu xfu v) True"
+  by (auto simp: xpres_abnormal_def creturn_def elim!: exec_elim_cases)
+
+lemma xpres_abnormal_creturn_void:
+  "xpres_abnormal \<Gamma> (creturn_void rtu) True"
+  by (auto simp: xpres_abnormal_def creturn_void_def elim!: exec_elim_cases)
+
+lemma xpres_abnormal_cbreak:
+  "xpres_abnormal \<Gamma> (cbreak rtu) True"
+  by (auto simp: xpres_abnormal_def cbreak_def elim!: exec_elim_cases)
+
+lemma xpres_abnormal_guard:
+  assumes "xpres_abnormal \<Gamma> c abnormal"
+  shows "xpres_abnormal \<Gamma> (Guard f g c) abnormal"
+  apply (rule xpres_abnormalI)
+  apply (erule exec_elim_cases; clarsimp; erule (1) assms[THEN xpres_abnormalD])
+  done
+
+lemma xpres_abnormal_seq:
+  assumes C: "xpres_abnormal \<Gamma> c C"
+             "xpres_abnormal \<Gamma> d D"
+  assumes S: "xpres_eq_If C True D S"
+  shows "xpres_abnormal \<Gamma> (Seq c d) S"
+  apply (rule xpres_abnormalI)
+  apply (erule exec_elim_cases; clarsimp)
+  apply (frule Normal_result, clarsimp, rename_tac s s')
+  apply (clarsimp simp: S[unfolded xpres_eq_If_def] if_bool_simps)
+  apply (erule disjE; erule (1) C[THEN xpres_abnormalD])
+  done
+
+lemma xpres_abnormal_cond:
+  assumes C: "xpres_abnormal \<Gamma> c C"
+             "xpres_abnormal \<Gamma> d D"
+  assumes S: "xpres_eq_If C D False S" (* S = (C \<and> D) *)
+  shows "xpres_abnormal \<Gamma> (Cond b c d) S"
+  apply (rule xpres_abnormalI)
+  apply (clarsimp simp: S[unfolded xpres_eq_If_def] if_bool_simps)
+  apply (erule exec_elim_cases; clarsimp; erule (1) C[THEN xpres_abnormalD])
+  done
+
+lemma xpres_abnormal_call:
+  assumes "\<And>s t. xpres_abnormal \<Gamma> (ret s t) abnormal"
+  shows "xpres_abnormal \<Gamma> (call i f reset ret) abnormal"
+  using assms by (auto simp: xpres_abnormal_def elim: exec_call_Normal_elim)
+
+lemmas xpres_abnormal_rules
+  = xpres_abnormal_creturn xpres_abnormal_creturn_void xpres_abnormal_cbreak xpres_abnormal_guard
+    xpres_abnormal_seq xpres_abnormal_cond xpres_abnormal_call
+
+(* Intended to be used to calculate `pres_norm`, `pres_abr` and `abnormal`
+   by syntactic analysis of `c`. *)
+definition xpres_strong ::
+  "('s,'p,'f) body \<Rightarrow> ('s \<Rightarrow> 'v) \<Rightarrow> 'v \<Rightarrow> ('s,'p,'f) com \<Rightarrow> bool \<Rightarrow> bool \<Rightarrow> bool \<Rightarrow> bool"
+  where
+  "xpres_strong \<Gamma> xf v c pres_norm pres_abr abnormal
+   \<equiv> (\<forall>s t. (\<Gamma> \<turnstile> \<langle>c, Normal s\<rangle> \<Rightarrow> Normal t \<longrightarrow> \<not> abnormal \<and> (pres_norm \<longrightarrow> xf s = v \<longrightarrow> xf t = v))
+          \<and> (\<Gamma> \<turnstile> \<langle>c, Normal s\<rangle> \<Rightarrow> Abrupt t \<longrightarrow> pres_abr \<longrightarrow> xf s = v \<longrightarrow> xf t = v))
+      \<and> (abnormal \<longrightarrow> pres_norm)"
+
+(* For compatibility with older proofs. *)
+abbreviation "xpres \<Gamma> xf v c \<equiv> xpres_strong \<Gamma> xf v c True True False"
+
+lemma xpres_def:
+  "xpres \<Gamma> xf v c \<equiv> \<forall>s t. \<Gamma> \<turnstile> \<langle>c, Normal s\<rangle> \<Rightarrow> t
+                          \<longrightarrow> xf s = v \<longrightarrow> (\<forall>t'. t = Normal t' \<or> t = Abrupt t' \<longrightarrow> xf t' = v)"
+  by (auto simp: xpres_strong_def atomize_eq)
+
+lemma xpres_strongI:
+  assumes "\<And>s t. \<lbrakk>pres_norm; \<Gamma> \<turnstile> \<langle>c, Normal s\<rangle> \<Rightarrow> Normal t; xf s = v\<rbrakk> \<Longrightarrow> xf t = v"
+  assumes "\<And>s t. \<lbrakk>pres_abr; \<Gamma> \<turnstile> \<langle>c, Normal s\<rangle> \<Rightarrow> Abrupt t; xf s = v\<rbrakk> \<Longrightarrow> xf t = v"
+  assumes "\<And>s t. \<lbrakk>abnormal; \<Gamma> \<turnstile> \<langle>c, Normal s\<rangle> \<Rightarrow> Normal t\<rbrakk> \<Longrightarrow> False"
+  assumes "abnormal \<Longrightarrow> pres_norm"
+  shows "xpres_strong \<Gamma> xf v c pres_norm pres_abr abnormal"
+  unfolding xpres_strong_def
+  by (intro allI impI conjI notI; erule assms)
+
+lemma xpres_strong_abnormalD:
+  "xpres_strong \<Gamma> xf v c pres_norm pres_abr abnormal \<Longrightarrow> abnormal \<Longrightarrow> pres_norm"
+  by (simp add: xpres_strong_def)
 
 lemma xpresI:
   "\<lbrakk>\<And>s t t'. \<lbrakk>\<Gamma> \<turnstile> \<langle>c, Normal s\<rangle> \<Rightarrow> t; xf s = v; t = Normal t' \<or> t = Abrupt t' \<rbrakk> \<Longrightarrow> xf t' = v\<rbrakk> \<Longrightarrow>
-  xpres xf v \<Gamma> c"
+  xpres \<Gamma> xf v c"
   unfolding xpres_def by auto
 
-(* Sometimes it's easier to reason syntactically --- the two are more or less equivalent, under the assumption
-  that c doesn't fault or get stuck *)
-lemma xpres_hoareI:
-  "\<Gamma> \<turnstile> {s. xf s = v } c {s. xf s = v} \<Longrightarrow> xpres xf v \<Gamma> c"
-  apply (rule xpresI)
-  apply (drule hoare_sound)
-  apply (simp add:HoarePartialDef.valid_def cvalid_def)
-  apply (drule spec, drule spec, drule (1) mp)
-  apply clarsimp
-  done
+lemma xpres_strong_abnormal_iff:
+  "xpres_strong \<Gamma> xf v c abnormal False abnormal \<longleftrightarrow> xpres_abnormal \<Gamma> c abnormal"
+  by (auto simp: xpres_strong_def xpres_abnormal_def)
 
 lemma xpres_skip:
-  "xpres xf v \<Gamma> Skip"
-  apply (rule xpres_hoareI)
-  apply rule
-  done
+  "xpres \<Gamma> xf v Skip"
+  by (rule xpresI; erule exec_Normal_elim_cases; simp)
 
-lemma xpres_basic:
-  assumes rl: "\<And>s. xf s = v \<Longrightarrow> xf (f s) = v"
-  shows "xpres xf v \<Gamma> (Basic f)"
-  apply (rule xpresI)
-  apply (drule rl)
-  apply (erule exec_Normal_elim_cases)
-  apply clarsimp
-  done
+lemma xpres_strong_basic':
+  assumes rl: "\<And>s. pres_norm \<Longrightarrow> xf s = v \<Longrightarrow> xf (f s) = v"
+  shows "xpres_strong \<Gamma> xf v (Basic f) pres_norm pres_abr False"
+  by (rule xpres_strongI; simp?; erule exec_Normal_elim_cases; clarsimp simp: rl)
 
-lemma xpres_exec0:
-  assumes xp: "xpres xf v \<Gamma> c"
-  and     ex: "\<Gamma> \<turnstile> \<langle>c, Normal s\<rangle> \<Rightarrow> y"
-  and     xy: "y = Normal s' \<or> y = Abrupt s'"
-  and     xf: "xf s = v"
-  shows   "xf s' = v"
-  using xp ex xy xf
-  unfolding xpres_def
+lemmas xpres_strong_basic = xpres_strong_basic'[where pres_abr=True]
+lemmas xpres_basic = xpres_strong_basic[where pres_norm=True, simplified]
+
+lemma xpres_basic_False:
+  "xpres_strong \<Gamma> xf v (Basic f) False True False"
+  by (rule xpres_strong_basic, simp)
+
+lemma xpres_exec_Normal:
+  assumes "xpres_strong \<Gamma> xf v c pres_norm pres_abr abnormal"
+  assumes pres_norm
+  assumes "\<Gamma> \<turnstile> \<langle>c, Normal s\<rangle> \<Rightarrow> Normal t"
+  assumes "xf s = v"
+  shows "xf t = v"
+  using assms unfolding xpres_strong_def
   apply -
-  apply (drule spec, drule spec, drule (1) mp)
-  apply (erule disjE)
-   apply (drule mp, simp)
-   apply simp
-  apply (drule mp, simp)
-  apply simp
+  by (drule (1) mp | erule allE conjE trivial)+
+
+lemma xpres_exec_Abrupt:
+  assumes xp: "xpres_strong \<Gamma> xf v c pres_norm pres_abr abnormal"
+  assumes pa: pres_abr
+  assumes ex: "\<Gamma> \<turnstile> \<langle>c, Normal s\<rangle> \<Rightarrow> Abrupt t"
+  assumes xf: "xf s = v"
+  shows   "xf t = v"
+  using assms unfolding xpres_strong_def
+  apply -
+  by (drule (1) mp | erule allE conjE trivial)+
+
+lemma xpres_exec_abnormal:
+  assumes "xpres_strong \<Gamma> xf v c pres_norm pres_abr abnormal"
+  assumes abnormal
+  assumes "\<Gamma> \<turnstile> \<langle>c, Normal s\<rangle> \<Rightarrow> Normal t"
+  shows "False"
+  using assms unfolding xpres_strong_def
+  apply -
+  by (drule (1) mp | erule allE conjE notE)+
+
+lemmas xpres_execs = xpres_exec_Normal xpres_exec_Abrupt
+
+(* If `b` never produces a `Normal` result, then we vacuously have that whenever
+   the sequence results in a `Normal` state, then `xf` is preserved. Together with
+   the rule for `Cond`, this is useful in situations like this:
+     IF condition THEN
+       \<acute>xf := modified_value ;;
+       return
+     FI ;;
+     // here, `xf` is still preserved.  *)
+lemma xpres_strong_seq:
+  assumes xpa: "xpres_strong \<Gamma> xf v c c_pres_norm c_pres_abr c_abnormal"
+  assumes xpb: "xpres_strong \<Gamma> xf v d d_pres_norm d_pres_abr d_abnormal"
+  notes xps = xpa xpb
+  \<comment> \<open>abnormal \<longleftrightarrow> c_abnormal \<or> d_abnormal\<close>
+  \<comment> \<open>pres_norm \<longleftrightarrow> c_pres_norm \<and> d_pres_norm \<or> abnormal\<close>
+  \<comment> \<open>pres_abr \<longleftrightarrow> c_pres_abr \<and> c_pres_norm \<and> d_pres_abr \<or> c_abnormal \<and> c_pres_abr\<close>
+  assumes ifs: "xpres_eq_If c_abnormal True d_abnormal abnormal"
+               "xpres_eq_If c_pres_norm d_pres_norm False cd_pres_norm"
+               "xpres_eq_If cd_pres_norm True abnormal pres_norm"
+               "xpres_eq_If c_pres_norm d_pres_abr False c_norm_d_pres_abr"
+               "xpres_eq_If c_pres_abr c_norm_d_pres_abr False cd_pres_abr"
+               "xpres_eq_If c_abnormal c_pres_abr False c_abnormal_pres_abr"
+               "xpres_eq_If cd_pres_abr True c_abnormal_pres_abr pres_abr"
+  shows "xpres_strong \<Gamma> xf v (c ;; d) pres_norm pres_abr abnormal"
+  unfolding ifs[simplified xpres_eq_If_def if_bool_simps]
+  apply (rule xpres_strongI
+         ; simp?
+         ; erule exec_Normal_elim_cases
+         ; erule Normal_resultE Abrupt_resultE
+         ; simp
+         ; elim disjE conjE exec_elim_cases)
+          apply (all \<open>(drule (1) xps[THEN xpres_exec_abnormal], simp)?\<close>)
+     apply (all \<open>(drule (2) xpres_execs[OF xpa])\<close>, simp_all)
+   apply (all \<open>(erule (2) xpres_execs[OF xpb])\<close>)
   done
-
-lemma xpres_exec:
-  assumes xp: "xpres xf v \<Gamma> c"
-  and     ex: "\<Gamma> \<turnstile> \<langle>c, Normal s\<rangle> \<Rightarrow> Normal s'"
-  and     xf: "xf s = v"
-  shows   "xf s' = v"
-  using xp ex xf by (auto intro: xpres_exec0)
-
-lemma xpresD:
-  assumes xf: "xf s = v"
-  and     xp: "xpres xf v \<Gamma> a"
-  and     ex: "\<Gamma> \<turnstile> \<langle>a, Normal s\<rangle> \<Rightarrow> Normal s'"
-  shows   "xf s' = v"
-  by (rule xpres_exec [OF xp ex]) fact+
-
-lemma xpres_abruptD:
-  assumes xf: "xf s = v"
-  and     xp: "xpres xf v \<Gamma> a"
-  and     ex: "\<Gamma> \<turnstile> \<langle>a, Normal s\<rangle> \<Rightarrow> Abrupt s'"
-  shows   "xf s' = v"
-  by (rule xpres_exec0 [OF xp ex], simp) fact+
 
 lemma xpres_seq:
-  assumes xa: "xpres xf v \<Gamma> a"
-  and     xb: "xpres xf v \<Gamma> b"
-  shows   "xpres xf v \<Gamma> (a ;; b)"
-  apply (rule xpresI)
-  apply (erule exec_Normal_elim_cases)
-  apply (erule disjE)
-   apply simp
-   apply (erule Normal_resultE)
-   apply simp
-   apply (drule (1) xpresD [OF _ xa])
-   apply (erule (1) xpresD [OF _ xb])
-  apply simp
-  apply (erule Abrupt_resultE)
-   apply simp
-   apply (drule (1) xpresD [OF _ xa])
-   apply (erule (1) xpres_abruptD [OF _ xb])
-  apply simp
-  apply (drule Abrupt_end, rule refl)
-  apply simp
-  apply (erule (1) xpres_abruptD [OF _ xa])
-  done
+  assumes xpa: "xpres \<Gamma> xf v a"
+  assumes xpb: "xpres \<Gamma> xf v b"
+  shows "xpres \<Gamma> xf v (a ;; b)"
+  by (rule xpres_strong_seq[OF xpa xpb] xpres_eq_If_rules)+
 
-lemma xpres_while0:
+lemma xpres_strong_while0:
   assumes ex: "\<Gamma>\<turnstile> \<langle>d,s\<rangle> \<Rightarrow> t"
-  and     xp: "xpres xf v \<Gamma> a"
+  and     xp: "xpres_strong \<Gamma> xf v a pres_norm pres_abr abnormal"
   and      d: "d = While b a"
   and      s: "s \<in> Normal ` {s. xf s = v} \<union> Abrupt ` {s. xf s = v}"
-  and      t: "t = Normal t' \<or> t = Abrupt t'"
+  and      t: "pres_norm \<and> t = Normal t' \<or> pres_norm \<and> pres_abr \<and> t = Abrupt t'"
   shows    "xf t' = v"
   using ex d s t
 proof (induct)
   case (WhileTrue s' b' c' t u)
   hence eqs: "b' = b" "c' = a" and xfs: "xf s' = v" by auto
-
   {
     fix w
-    assume tv: "t = Normal w" and "\<Gamma> \<turnstile> \<langle>a, Normal s'\<rangle> \<Rightarrow> Normal w"
+    assume tv: "t = Normal w" and "\<Gamma> \<turnstile> \<langle>a, Normal s'\<rangle> \<Rightarrow> Normal w" and pres_norm
 
     have ?thesis
     proof (rule WhileTrue.hyps(5))
-      have "xf w = v" using xfs xp by (rule xpresD) fact+
+      have "xf w = v" by (rule xpres_exec_Normal) fact+
       thus "t \<in> Normal ` {s. xf s = v} \<union> Abrupt ` {s. xf s = v}" using tv
         by simp
     qed fact+
   } moreover
   {
     fix w
-    assume tv: "t = Abrupt w" and "\<Gamma> \<turnstile> \<langle>a, Normal s'\<rangle> \<Rightarrow> Abrupt w"
+    assume tv: "t = Abrupt w" and "\<Gamma> \<turnstile> \<langle>a, Normal s'\<rangle> \<Rightarrow> Abrupt w" and pres_abr
     have ?thesis
     proof (rule WhileTrue.hyps(5))
-      have "xf w = v" using xfs xp by (rule xpres_abruptD) fact+
+      have "xf w = v" by (rule xpres_exec_Abrupt) fact+
       thus "t \<in> Normal ` {s. xf s = v} \<union> Abrupt ` {s. xf s = v}" using tv
         by simp
     qed fact+
   } ultimately
-  show ?thesis using WhileTrue.prems(3) WhileTrue.hyps(2) WhileTrue.hyps(4) eqs
+  show ?thesis using WhileTrue.prems(3) WhileTrue.hyps(2) WhileTrue.hyps(4) unfolding eqs
   apply -
-  apply (erule disjE)
-   apply simp
-   apply (erule Normal_resultE)
-   apply simp
-  apply simp
-  apply (erule Abrupt_resultE)
-  apply simp
-  apply simp
-  done
+  by (elim disjE conjE; simp; erule Normal_resultE Abrupt_resultE; simp)
 qed auto
 
-lemma xpres_while:
-  assumes xp: "xpres xf v \<Gamma> x"
-  shows   "xpres xf v \<Gamma> (While b x)"
-  apply (rule xpresI)
-  apply (erule xpres_while0 [OF _ xp refl])
-   apply simp
-  apply simp
-  done
+lemma xpres_strong_while:
+  assumes xp: "xpres_strong \<Gamma> xf v x pres_norm pres_abr abnormal"
+  assumes pa: "xpres_eq_If pres_norm pres_abr False pres_abr'"
+  shows   "xpres_strong \<Gamma> xf v (While b x) pres_norm pres_abr' False"
+  unfolding pa[simplified xpres_eq_If_def if_bool_simps]
+  apply (rule xpres_strongI)
+  apply (erule xpres_strong_while0[OF _ xp refl]; simp)+
+  by auto
 
-lemma xpres_call_hoarep_gen:
+lemmas xpres_while
+  = xpres_strong_while[OF _ xpres_eq_If_True, where pres_abr=True and abnormal=False, simplified]
+
+lemma xpres_strong_xpres_abnormalI:
+  assumes abn: "xpres_strong \<Gamma> xf v c' pres_norm pres_abr' abnormal"
+  assumes "\<And>s t. \<lbrakk>pres_norm; \<Gamma> \<turnstile> \<langle>c, Normal s\<rangle> \<Rightarrow> Normal t; xf s = v\<rbrakk> \<Longrightarrow> xf t = v"
+  assumes "\<And>s t. \<lbrakk>pres_abr; \<Gamma> \<turnstile> \<langle>c, Normal s\<rangle> \<Rightarrow> Abrupt t; xf s = v\<rbrakk> \<Longrightarrow> xf t = v"
+  assumes "\<And>s t. \<lbrakk>abnormal; \<Gamma> \<turnstile> \<langle>c, Normal s\<rangle> \<Rightarrow> Normal t\<rbrakk> \<Longrightarrow> False"
+  shows "xpres_strong \<Gamma> xf v c pres_norm pres_abr abnormal"
+  by (rule xpres_strongI[OF _ _ _ xpres_strong_abnormalD[OF abn]]; erule assms trivial; assumption)
+
+lemma xpres_strong_call_hoarep_gen:
   assumes mod: "\<forall>s. \<Gamma>\<turnstile>\<^bsub>/F s\<^esub> (P s) Call f (Q s),(A s)"
-  assumes ret: "\<And>s t. xf s = v \<Longrightarrow> i s \<in> P (x s) \<longrightarrow> t \<in> Q (x s) \<or> t \<in> A (x s) \<Longrightarrow> xf (r s t) = v"
-  assumes xpr: "\<And>s t. xpres xf v \<Gamma> (c s t)"
-  shows "xpres xf v \<Gamma> (call i f r c)"
-  apply (rule xpresI)
-  apply (erule exec_call_Normal_elim)
-      apply (erule (1) xpres_exec0[OF xpr])
-      apply (erule ret)
-      apply (frule (1) hoarep_exec_call_body[OF mod], fastforce)
-     apply simp
-     apply (erule subst, erule ret)
+  assumes ret: "\<And>s t. xf s = v \<Longrightarrow> i s \<in> P (x s) \<longrightarrow> t \<in> Q (x s) \<or> t \<in> A (x s) \<Longrightarrow> xf (reset s t) = v"
+  assumes xpr: "\<And>s t. xpres_strong \<Gamma> xf v (ret s t) pres_norm pres_abr abnormal"
+  shows "xpres_strong \<Gamma> xf v (call i f reset ret) pres_norm pres_abr abnormal"
+  apply (rule xpres_strong_xpres_abnormalI[OF xpr]; simp?; erule exec_call_Normal_elim; simp?)
+     apply (erule (1) xpres_execs[OF xpr])
+     apply (erule ret)
      apply (frule (1) hoarep_exec_call_body[OF mod], fastforce)
-    apply simp
-   apply simp
-  apply simp
+    apply (erule (1) xpres_execs[OF xpr])
+    apply (erule ret)
+    apply (frule (1) hoarep_exec_call_body[OF mod], fastforce)
+   apply (erule ret)
+   apply (frule (1) hoarep_exec_call_body[OF mod], fastforce)
+  apply (erule (1) xpres_exec_abnormal[OF xpr])
   done
 
-lemmas xpres_call = xpres_call_hoarep_gen[OF hoarep_false_pre_gen, simplified]
-lemmas xpres_call_hoarep = xpres_call_hoarep_gen[where P="\<lambda>s. {s}" and x=i and i=i for i, simplified]
+lemmas xpres_call = xpres_strong_call_hoarep_gen[OF hoarep_false_pre_gen, simplified]
+lemmas xpres_call_hoarep = xpres_strong_call_hoarep_gen[where P="\<lambda>s. {s}" and x=i and i=i for i, simplified]
+
+lemma xpres_strong_catch:
+  assumes xpc: "xpres_strong \<Gamma> xf v c c_pres_norm c_pres_abr c_abnormal"
+  assumes xpd: "xpres_strong \<Gamma> xf v d d_pres_norm d_pres_abr d_abnormal"
+  notes xps = xpc xpd
+  \<comment> \<open>abnormal \<longleftrightarrow> c_abnormal \<and> d_abnormal\<close>
+  \<comment> \<open>pres_norm \<longleftrightarrow> abnormal \<or> c_pres_norm \<and> c_pres_abr \<and> d_pres_norm\<close>
+  \<comment> \<open>pres_abr \<longleftrightarrow> c_pres_abr \<and> c_pres_abr\<close>
+  assumes rew: "xpres_eq_If c_abnormal d_abnormal False abnormal"
+               "xpres_eq_If c_pres_norm c_pres_abr False c_pres_norm_abr"
+               "xpres_eq_If c_pres_norm_abr d_pres_norm False cd_pres_norm"
+               "xpres_eq_If abnormal True cd_pres_norm pres_norm"
+               "xpres_eq_If c_pres_abr d_pres_abr False pres_abr"
+  shows "xpres_strong \<Gamma> xf v (Catch c d) pres_norm pres_abr abnormal"
+  unfolding rew[simplified xpres_eq_If_def if_bool_simps]
+  apply (rule xpres_strongI; simp?; erule exec_Normal_elim_cases; simp?; (elim disjE conjE)?)
+          apply (all \<open>(drule (1) xps[THEN xpres_exec_abnormal], simp)?\<close>)
+     apply (all \<open>drule (2) xpres_execs[OF xpc], assumption?\<close>)
+   apply (all \<open>drule (2) xpres_execs[OF xpd], assumption\<close>)
+  done
 
 lemma xpres_catch:
-  assumes xpb: "xpres xf v \<Gamma> b"
-  and     xpc: "xpres xf v \<Gamma> c"
-  shows    "xpres xf v \<Gamma> (Catch b c)"
-  apply (rule xpresI)
-  apply (erule exec_Normal_elim_cases)
-   apply (drule (1) xpres_abruptD [OF _ xpb])
-   apply (erule (2) xpres_exec0 [OF xpc])
-  apply (erule (2) xpres_exec0 [OF xpb])
+  assumes "xpres \<Gamma> xf v b"
+  assumes "xpres \<Gamma> xf v c"
+  shows "xpres \<Gamma> xf v (Catch b c)"
+  by (rule xpres_strong_catch[OF assms] xpres_eq_If_rules)+
+
+lemma xpres_strong_guard:
+  assumes "xpres_strong \<Gamma> xf v c pres_norm pres_abr abnormal"
+  shows "xpres_strong \<Gamma> xf v (Guard f g c) pres_norm pres_abr abnormal"
+  apply (rule xpres_strong_xpres_abnormalI[OF assms]; erule exec_Normal_elim_cases; simp?)
+     apply (all \<open>drule (1) xpres_execs[OF assms] assms[THEN xpres_exec_abnormal]; simp\<close>)
   done
 
-lemma xpres_guard:
-  assumes xp: "xpres xf v \<Gamma> c"
-  shows   "xpres xf v \<Gamma> (Guard f g c)"
-  apply (rule xpresI)
-  apply (erule exec_Normal_elim_cases)
-   apply (erule (2) xpres_exec0 [OF xp])
-  apply simp
+lemmas xpres_guard = xpres_strong_guard[where pres_norm=True and pres_abr=True and abnormal=False]
+
+lemma xpres_strong_cond:
+  assumes xpc: "xpres_strong \<Gamma> xf v c c_pres_norm c_pres_abr c_abnormal"
+  assumes xpd: "xpres_strong \<Gamma> xf v d d_pres_norm d_pres_abr d_abnormal"
+  notes xps = xpc xpd
+  \<comment> \<open>pres_norm \<longleftrightarrow> abnormal \<or> c_pres_norm \<and> d_pres_norm \<or> c_abnormal \<and> d_pres_norm \<or> c_pres_norm \<and> d_abnormal\<close>
+  \<comment> \<open>pres_abr \<longleftrightarrow> c_pres_abr \<and> d_pres_abr\<close>
+  \<comment> \<open>abnormal \<longleftrightarrow> c_abnormal \<and> d_abnormal\<close>
+  assumes rew: "xpres_eq_If c_abnormal d_abnormal False abnormal"
+               "xpres_eq_If c_pres_norm d_pres_norm False cd_pres_norm"
+               "xpres_eq_If c_abnormal d_pres_norm False ca_pres_norm"
+               "xpres_eq_If c_pres_norm d_abnormal False da_pres_norm"
+               "xpres_eq_If ca_pres_norm True da_pres_norm cda_pres_norm"
+               "xpres_eq_If cd_pres_norm True cda_pres_norm pres_norm'"
+               "xpres_eq_If abnormal True pres_norm' pres_norm"
+               "xpres_eq_If c_pres_abr d_pres_abr False pres_abr"
+  shows "xpres_strong \<Gamma> xf v (Cond x c d) pres_norm pres_abr abnormal"
+  unfolding rew[simplified xpres_eq_If_def if_bool_simps]
+  apply (rule xpres_strongI; simp?; erule exec_Normal_elim_cases; elim disjE conjE)
+             apply (all \<open>(drule (1) xps[THEN xpres_exec_abnormal], simp)?\<close>)
+       apply (all \<open>(erule (2) xpres_execs[OF xpc] xpres_execs[OF xpd])\<close>)
   done
 
 lemma xpres_cond:
-  assumes xpa: "xpres xf v \<Gamma> a"
-  and     xpb: "xpres xf v \<Gamma> b"
-  shows   "xpres xf v \<Gamma> (Cond x a b)"
-  apply (rule xpresI)
-  apply (erule exec_Normal_elim_cases)
-   apply (erule (2) xpres_exec0 [OF xpa])
-  apply (erule (2) xpres_exec0 [OF xpb])
-  done
+  assumes "xpres \<Gamma> xf v a"
+  assumes "xpres \<Gamma> xf v b"
+  shows "xpres \<Gamma> xf v (Cond x a b)"
+  by (rule xpres_strong_cond[OF assms] xpres_eq_If_rules)+
 
-lemma xpres_throw:
-  shows   "xpres xf v \<Gamma> Throw"
-  apply (rule xpresI)
-  apply (erule exec_Normal_elim_cases)
-  apply simp
-  done
+lemma xpres_strong_throw':
+  shows   "xpres_strong \<Gamma> xf v Throw True True abnormal"
+  by (rule xpres_strongI; simp?; erule exec_Normal_elim_cases; simp)
 
-lemma xpres_creturn:
-  assumes xfu: "\<And>s f. xf (xfu f s) = xf s"
-  and xfg: "\<And>s f. xf (exnu f s) = xf s"
-  shows   "xpres xf v \<Gamma> (creturn exnu xfu v')"
+lemmas xpres_strong_throw = xpres_strong_throw'[where abnormal=True]
+lemmas xpres_throw = xpres_strong_throw'[where abnormal=False]
+
+lemma xpres_strong_creturn':
+  assumes xfu: "\<And>s f. pres_abr \<Longrightarrow> xf (xfu f s) = xf s"
+  and xfg: "\<And>s f. pres_abr \<Longrightarrow> xf (exnu f s) = xf s"
+  shows   "xpres_strong \<Gamma> xf v (creturn exnu xfu v') True pres_abr abnormal"
   unfolding creturn_def
-  apply (rule xpresI)
-  apply (clarsimp elim!: exec_Normal_elim_cases simp add: xfg xfu)+
-  done
+  by (rule xpres_strongI; clarsimp elim!: exec_Normal_elim_cases simp: xfu xfg)
 
-lemma xpres_creturn_void:
-  assumes xfg: "\<And>s f. xf (exnu f s) = xf s"
-  shows   "xpres xf v \<Gamma> (creturn_void exnu)"
+lemmas xpres_strong_creturn = xpres_strong_creturn'[where pres_abr=True and abnormal=True, simplified]
+lemmas xpres_strong_creturn_False = xpres_strong_creturn'[where pres_abr=False and abnormal=True, simplified]
+lemmas xpres_creturn = xpres_strong_creturn'[where pres_abr=True and abnormal=False, simplified]
+
+lemma xpres_strong_creturn_void':
+  assumes xfg: "\<And>s f. pres_abr \<Longrightarrow> xf (exnu f s) = xf s"
+  shows   "xpres_strong \<Gamma> xf v (creturn_void exnu) True pres_abr abnormal"
   unfolding creturn_void_def
-  apply (rule xpresI)
-  apply (clarsimp elim!: exec_Normal_elim_cases simp add: xfg)
-  done
+  by (rule xpres_strongI; clarsimp elim!: exec_Normal_elim_cases simp: xfg)
 
-lemma xpres_cbreak:
-  assumes xfg: "\<And>s f. xf (exnu f s) = xf s"
-  shows   "xpres xf v \<Gamma> (cbreak exnu)"
+lemmas xpres_strong_creturn_void = xpres_strong_creturn_void'[where pres_abr=True and abnormal=True, simplified]
+lemmas xpres_strong_creturn_void_False = xpres_strong_creturn_void'[where pres_abr=False and abnormal=True, simplified]
+lemmas xpres_creturn_void = xpres_strong_creturn_void'[where pres_abr=True and abnormal=False, simplified]
+
+lemma xpres_strong_cbreak':
+  assumes xfg: "\<And>s f. pres_abr \<Longrightarrow> xf (exnu f s) = xf s"
+  shows   "xpres_strong \<Gamma> xf v (cbreak exnu) True pres_abr abnormal"
   unfolding cbreak_def
-  apply (rule xpresI)
-  apply (clarsimp elim!: exec_Normal_elim_cases simp add: xfg)
-  done
+  by (rule xpres_strongI; clarsimp elim!: exec_Normal_elim_cases simp add: xfg)
+
+lemmas xpres_strong_cbreak = xpres_strong_cbreak'[where pres_abr=True and abnormal=True, simplified]
+lemmas xpres_strong_cbreak_False = xpres_strong_cbreak'[where pres_abr=False and abnormal=True, simplified]
+lemmas xpres_cbreak = xpres_strong_cbreak'[where pres_abr=True and abnormal=False, simplified]
 
 lemma xpres_catchbrk_C:
-  shows   "xpres xf v \<Gamma> (ccatchbrk exnu)"
+  shows   "xpres \<Gamma> xf v (ccatchbrk exnu)"
   unfolding ccatchbrk_def
-  apply (rule xpresI)
-  apply (fastforce elim!: exec_Normal_elim_cases)
-  done
+  by (rule xpresI; fastforce elim!: exec_Normal_elim_cases)
 
-lemma xpres_lvar_nondet_init:
-  assumes xfg: "\<And>s f. xf (st f s) = xf s"
-  shows   "xpres xf v \<Gamma> (lvar_nondet_init gt st)"
-  apply (rule xpresI)
-  apply (simp add: lvar_nondet_init_def)
-  apply (auto elim!: exec_Normal_elim_cases simp add: xfg)
-  done
+lemma xpres_strong_lvar_nondet_init:
+  assumes xfg: "\<And>s f. pres_norm \<Longrightarrow> xf (st f s) = xf s"
+  shows   "xpres_strong \<Gamma> xf v (lvar_nondet_init gt st) pres_norm True False"
+  by (auto intro!: xpres_strongI elim!: exec_Normal_elim_cases simp: xfg lvar_nondet_init_def)
+
+lemmas xpres_lvar_nondet_init_False = xpres_strong_lvar_nondet_init[where pres_norm=False, simplified]
+lemmas xpres_lvar_nondet_init = xpres_strong_lvar_nondet_init[where pres_norm=True, simplified]
 
 (* We ignore DynCom and Call and (for now) Spec.  The first two are covered by xpres_call *)
 lemmas xpres_rules = xpres_skip xpres_basic xpres_seq xpres_while
